converted most of mso to permutation up to an equivalence

mso.v
@@ -79,7 +79,7 @@ Section utilities.
 End utilities.
 
 Fact Forall2_middle_inv_left X Y (R : X → Y → Prop) l x r m :
-  Forall2 R (l++[x]++r) m → ∃ l' y r', m = l'++[y]++r' ∧ Forall2 R l l' ∧ Forall2 R r r'.
+  Forall2 R (l++[x]++r) m → ∃ l' y r', m = l'++[y]++r' ∧ R x y ∧ Forall2 R l l' ∧ Forall2 R r r'.
 Proof.
   intros (l' & [ | y r' ] & H1 & H2 & ->)%Forall2_app_inv_l.
   1: now inversion H2.
@@ -146,7 +146,7 @@ Proof.
 Qed.
 
 Fact perm_Forall2_xchg [X Y] [E : X → Y → Prop] [l m k] :
-  l ~ₚ m → Forall2 E m k →  ∃p, Forall2 E l p ∧ p ~ₚ k.
+  l ~ₚ m → Forall2 E m k → ∃p, Forall2 E l p ∧ p ~ₚ k.
 Proof.
   intros H1%Permutation_sym H2%Forall2_xchg.
   destruct (Forall2_perm_xchg H2 H1) as (? & ? & ?%Forall2_xchg); eauto.
@@ -158,8 +158,8 @@ Section perm_eq.
 
   Implicit Type (E : X → X → Prop).
 
-  Inductive perm_eq E : list X → list X → Prop :=
-    | perm_eq_intro l m k : Forall2 E l m → m ~ₚ k → perm_eq E l k.
+  Inductive perm_eq E (l k : list X) : Prop :=
+    | perm_eq_intro m : Forall2 E l m → m ~ₚ k → perm_eq E l k.
 
   Hint Constructors perm_eq : core.
 
@@ -174,7 +174,7 @@ Section perm_eq.
 
   Fact perm_eq_xchg E l m : perm_eq E l m → ∃p, l ~ₚ p ∧ Forall2 E p m.
   Proof.
-    destruct 1 as [ l m k H1 H2 ].
+    destruct 1 as [ k H1 H2 ].
     apply (Forall2_perm_xchg H1 H2).
   Qed.
 
@@ -198,23 +198,98 @@ Section perm_eq.
   Proof.
     intros Hlmk.
     intros (u & H1 & H2)%perm_eq_xchg.
-    destruct 1 as [ m v k H3 H4 ].
+    destruct 1 as [ v H3 H4 ].
     assert (Forall2 E u v) as Huv.
     1: revert H2 H3; apply Forall2_trans_dep; eauto.
     destruct (perm_Forall2_xchg H1 Huv) as (? & []); eauto.
+  Qed.
+
+  Hint Resolve Forall2_app : core.
+
+  Fact perm_eq_app E l m k p : perm_eq E l m → perm_eq E k p → perm_eq E (l++k) (m++p).
+  Proof. do 2 destruct 1; eauto. Qed.
+
+  Hint Resolve Forall2_app : core.
+
+  Fact perm_eq_app_comm E l m :
+      (∀x, x ∈ l → E x x)
+    → (∀x, x ∈ m → E x x)
+    → perm_eq E (l++m) (m++l).
+  Proof.
+    rewrite <- !Forall_forall.
+    intros H1 H2.
+    constructor 1 with (l++m).
+    + apply Forall2_app.
+      * induction H1; eauto.
+      * induction H2; eauto.
+    + apply Permutation_app_comm.
+  Qed. 
+
+  Fact perm_eq_middle_inv E l x r m : 
+      perm_eq E (l++[x]++r) m 
+    → ∃ l' y r', E x y 
+               ∧ m = l'++[y]++r' 
+               ∧ perm_eq E (l++r) (l'++r').
+  Proof.
+    destruct 1 as [ v (l1 & y & r1 & -> & H1 & H2 & H3)%Forall2_middle_inv_left 
+                    (l' & r' & -> & H)%Permutation_middle_inv ].
+    exists l', y, r'; repeat split; auto.
+    constructor 1 with (l1++r1); eauto.
   Qed.
 
 End perm_eq.
 
 Section multiset_order.
 
-  Variables (X : Type) (R : X → X → Prop).
+  Variables (X : Type) (R E : X → X → Prop).
 
   (* Infix notation for the base relation *)
   Infix "<" := R.
+  Notation "x ≃ y" := (E x y) (at level 70).
+  Notation "x ~ₑ y" := (perm_eq E x y) (at level 70).
+
+  Hypothesis E_refl : reflexive _ E.
+  Hypothesis E_sym  : symmetric _ E.
+  Hypothesis E_trans : transitive _ E.
+
+  Hypothesis E_R_comp : ∀ x a b, a ≃ b → x < a → x < b.
 
   (* x is a <-upper bound for the list m *)
   Notation "m <ₗ x" := (∀y, y ∈ m → y < x).
+
+  Local Fact perm_E_refl l : l ~ₑ l.
+  Proof. apply perm_eq_refl; auto. Qed.
+
+  Local Fact perm_E_sym l m : l ~ₑ m → m ~ₑ l.
+  Proof. apply perm_eq_sym; auto. Qed.
+
+  Local Fact perm_E_trans l m k : l ~ₑ m → m ~ₑ k → l ~ₑ k.
+  Proof. apply perm_eq_trans; eauto. Qed.
+
+  Local Fact perm_E_app l m p q : l ~ₑ m → p ~ₑ q → l++p ~ₑ m++q.
+  Proof. apply perm_eq_app. Qed.
+
+  Hint Resolve perm_E_refl perm_E_sym perm_E_trans perm_E_app : core.
+
+  Local Fact perm_E_app_comm l m : l++m ~ₑ m++l.
+  Proof. apply perm_eq_app_comm; auto. Qed.
+
+  Local Fact E_bound_comp l x y : x ≃ y → l <ₗ x → l <ₗ y.
+  Proof. intros ? ? ? ?; eauto. Qed.
+
+  Hint Resolve perm_E_app_comm E_bound_comp : core.
+
+  Local Fact perm_E_middle l m r l' r' :
+    l++r ~ₑ l'++r' → l++m++r ~ₑ l'++m++r'.
+  Proof.
+    intros H.
+    do 2 apply perm_E_trans with (1 := perm_E_app_comm _ _), perm_E_sym.
+    rewrite <- ! app_assoc.
+    apply perm_E_app; auto.
+    now do 2 apply perm_E_trans with (1 := perm_E_app_comm _ _), perm_E_sym.
+  Qed.
+
+  Hint Resolve perm_E_middle : core.
 
   (* Inductive definition of the list/multiset relation ⊏
      of which the transitive closure ⊏⁺ is the mso. The
@@ -224,7 +299,7 @@ Section multiset_order.
   Inductive mso_step : list X → list X → Prop :=
     | mso_step_intro l m x r : m <ₗ x 
                              → l++m++r ⊏ l++[x]++r
-    | mso_step_perm_l l m k  : l ~ₚ m
+    | mso_step_perm_l l m k  : l ~ₑ m
                              → l ⊏ k
                              → m ⊏ k
   where "l ⊏ m" := (mso_step l m).
@@ -233,7 +308,7 @@ Section multiset_order.
 
   (* The inversion lemma gives an alternate FO characterization *)
   Fact mso_step_inv k p : 
-     k ⊏ p ↔ ∃ l m x r, k ~ₚ l++m++r ∧ p = l++[x]++r ∧ m <ₗ x.
+     k ⊏ p ↔ ∃ l m x r, k ~ₑ l++m++r ∧ p = l++[x]++r ∧ m <ₗ x.
   Proof.
     split.
     + induction 1 as [ | ? ? ? ? ? (? & ? & ? & ? & ? & -> & ?) ]; do 4 eexists; eauto.
@@ -255,11 +330,12 @@ Section multiset_order.
   Qed.
 
   (* ⊏ is closed under right permutation *)
-  Fact mso_step_perm_r l m k : l ~ₚ m → k ⊏ l → k ⊏ m.
+  Fact mso_step_perm_r l m k : l ~ₑ m → k ⊏ l → k ⊏ m.
   Proof.
     intros H1 H2; revert H2 m H1.
     induction 1; intro; eauto.
-    intros (? & ? & -> & ?)%Permutation_middle_inv; eauto.
+    intros (? & ? & ? & ? & -> & ?)%perm_eq_middle_inv; eauto.
+    constructor 2 with (x0++m++x2); eauto.
   Qed.
 
   Fact mso_step_cons x l : l ⊏ x::l.
@@ -278,10 +354,10 @@ Section multiset_order.
        Acc_mso_step below *)
   Lemma mso_step_cons_right_inv k y m : 
       k ⊏ y::m 
-    → (∃ u,       k ~ₚ u ++ m 
+    → (∃ u,       k ~ₑ u ++ m 
                 ∧ u <ₗ y)
     ∨ (∃ l u x r, m = l++[x]++r
-                ∧ k ~ₚ y::l++u++r
+                ∧ k ~ₑ y::l++u++r
                 ∧ u <ₗ x).
   Proof.
     intros ([] & ? & ? & ? & ? & [-> ->]%cons_inj & ?)%mso_step_inv; simpl in *. 
@@ -296,7 +372,7 @@ Section multiset_order.
 
     Notation W := (Acc mso_step).
 
-    Local Fact Permutation_Acc_mso_step l m : l ~ₚ m → W m → W l.
+    Local Fact Permutation_Acc_mso_step l m : l ~ₑ m → W m → W l.
     Proof. intros ? []; eauto. Qed.
 
     Local Fact Acc_mso_step_nil : W [].
@@ -381,10 +457,10 @@ Section multiset_order.
 
   (* Closure under left/right permutations *)
 
-  Fact mso_perm_l l m k : l ~ₚ m → l ⊏⁺ k → m ⊏⁺ k.
+  Fact mso_perm_l l m k : l ~ₑ m → l ⊏⁺ k → m ⊏⁺ k.
   Proof. unfold mso; intros H1 H2; revert m H1; induction H2; eauto. Qed.
 
-  Fact mso_perm_r l m k : l ~ₚ m → k ⊏⁺ l → k ⊏⁺ m.
+  Fact mso_perm_r l m k : l ~ₑ m → k ⊏⁺ l → k ⊏⁺ m.
   Proof. unfold mso; intros H1 H2; revert m H1; induction H2; eauto. Qed.
 
   Hint Resolve mso_step_cons mso_trans : core.
@@ -396,9 +472,8 @@ Section multiset_order.
   Fact mso_app_tail l m r : m ⊏⁺ l → m ⊏⁺ l++r.
   Proof.
     intros H.
-    apply mso_perm_r with (r++l).
-    + apply Permutation_app_comm.
-    + now apply mso_app_head.
+    apply mso_perm_r with (r++l); auto.
+    now apply mso_app_head.
   Qed.
 
   (* [] is also minimal for ⊏⁺ *)
